Hoare/HoareTripleForInstructions3.thy
@@ -68,7 +68,7 @@ inductive triple_inst_arith :: "pred \<Rightarrow> pos_inst \<Rightarrow> pred \
   inst_arith_2_1_low :
     "i \<in> {MUL, DIV, MOD} \<Longrightarrow>
 		triple_inst_arith
-      (\<langle> h \<le> 1022 \<and> Glow \<le> g \<and> m \<ge> 0\<rangle> **
+      (\<langle> h \<le> 1022 \<and> Glow \<le> g \<and> m \<ge> 0\<rangle> \<and>*
        continuing \<and>* memory_usage m \<and>* program_counter n \<and>*
        stack_height (Suc (Suc h)) \<and>* stack (Suc h) v \<and>* stack h w \<and>*
 			 gas_pred g \<and>* rest)
@@ -80,7 +80,7 @@ inductive triple_inst_arith :: "pred \<Rightarrow> pos_inst \<Rightarrow> pred \
 |  inst_arith_2_1_verylow :
     "i \<in> {ADD, SUB, inst_GT, inst_EQ, inst_LT} \<Longrightarrow>
 		 triple_inst_arith
-      (\<langle> h \<le> 1022 \<and> Gverylow \<le> g \<and> m \<ge> 0\<rangle> **
+      (\<langle> h \<le> 1022 \<and> Gverylow \<le> g \<and> m \<ge> 0\<rangle> \<and>*
        continuing \<and>* memory_usage m \<and>* program_counter n \<and>*
        stack_height (Suc (Suc h)) \<and>* stack (Suc h) v \<and>* stack h w \<and>*
 			 gas_pred g \<and>* rest)
@@ -92,7 +92,7 @@ inductive triple_inst_arith :: "pred \<Rightarrow> pos_inst \<Rightarrow> pred \
 |  inst_arith_3_1 :
     "i \<in> {ADDMOD, MULMOD} \<Longrightarrow>
 		 triple_inst_arith
-      (\<langle> h \<le> 1021 \<and> Gmid \<le> g \<and> m \<ge> 0\<rangle> **
+      (\<langle> h \<le> 1021 \<and> Gmid \<le> g \<and> m \<ge> 0\<rangle> \<and>*
        continuing \<and>* memory_usage m \<and>* program_counter n \<and>*
        stack_height (Suc (Suc (Suc h))) \<and>* stack (Suc (Suc h)) u \<and>* stack (Suc h) v \<and>* stack h w \<and>*
 			 gas_pred g \<and>* rest)
@@ -103,7 +103,7 @@ inductive triple_inst_arith :: "pred \<Rightarrow> pos_inst \<Rightarrow> pred \
        gas_pred (g - Gmid) \<and>* rest)"
 | inst_iszero :
     "triple_inst_arith
-      (\<langle> h \<le> 1023 \<and> Gverylow \<le> g \<and> m \<ge> 0\<rangle> **
+      (\<langle> h \<le> 1023 \<and> Gverylow \<le> g \<and> m \<ge> 0\<rangle> \<and>*
        continuing \<and>* memory_usage m \<and>* program_counter n \<and>*
        stack_height (Suc h) \<and>* stack h w \<and>* gas_pred g \<and>* rest)
       (n, Arith ISZERO)
@@ -122,7 +122,7 @@ fun bits_2_1_verylow:: "bits_inst \<Rightarrow> w256 \<Rightarrow> w256 \<Righta
 inductive triple_inst_bits :: "pred \<Rightarrow> pos_inst \<Rightarrow> pred \<Rightarrow> bool" where
   inst_instNOT :
     "triple_inst_bits
-      (\<langle> h \<le> 1023 \<and> Gverylow \<le> g \<and> m \<ge> 0\<rangle> **
+      (\<langle> h \<le> 1023 \<and> Gverylow \<le> g \<and> m \<ge> 0\<rangle> \<and>*
        continuing \<and>* memory_usage m \<and>* program_counter n \<and>*
        stack_height (Suc h) \<and>* stack h w \<and>* gas_pred g \<and>* rest)
       (n, Bits inst_NOT)
@@ -133,7 +133,7 @@ inductive triple_inst_bits :: "pred \<Rightarrow> pos_inst \<Rightarrow> pred \<
 |  inst_bits_2_1_verylow :
     "i \<in> {inst_AND, inst_OR, inst_XOR, BYTE} \<Longrightarrow>
 		 triple_inst_bits
-      (\<langle> h \<le> 1022 \<and> Gverylow \<le> g \<and> m \<ge> 0\<rangle> **
+      (\<langle> h \<le> 1022 \<and> Gverylow \<le> g \<and> m \<ge> 0\<rangle> \<and>*
        continuing \<and>* memory_usage m \<and>* program_counter n \<and>*
        stack_height (Suc (Suc h)) \<and>* stack (Suc h) v \<and>* stack h w \<and>*
 			 gas_pred g \<and>* rest)
@@ -155,7 +155,7 @@ inductive triple_inst_pc :: "pred \<Rightarrow> pos_inst \<Rightarrow> pred \<Ri
        gas_pred (g - Gjumpdest) \<and>* rest)"
 | inst_pc :
     "triple_inst_pc
-      (\<langle> h \<le> 1023 \<and> Gbase \<le> g \<and> m \<ge> 0\<rangle> **
+      (\<langle> h \<le> 1023 \<and> Gbase \<le> g \<and> m \<ge> 0\<rangle> \<and>*
        continuing \<and>* memory_usage m \<and>* program_counter n \<and>*
        stack_height h \<and>* gas_pred g \<and>* rest)
       (n, Pc PC)
@@ -178,13 +178,23 @@ inductive triple_inst_stack :: "pred \<Rightarrow> pos_inst \<Rightarrow> pred \
        stack h (word_rcat lst) \<and>* rest)"
 | inst_pop :
     "triple_inst_stack
-      (\<langle> h \<le> 1023 \<and> Gbase \<le> g \<and> m \<ge> 0\<rangle> **
+      (\<langle> h \<le> 1023 \<and> Gbase \<le> g \<and> m \<ge> 0\<rangle> \<and>*
        continuing \<and>* memory_usage m \<and>* program_counter n \<and>*
        stack_height (Suc h) \<and>* stack h w \<and>* gas_pred g \<and>* rest)
       (n, Stack POP)
       (program_counter (n + 1) \<and>* continuing \<and>*
        memory_usage m \<and>* stack_height h \<and>*
        gas_pred (g - Gbase) \<and>* rest)"
+| inst_calldataload :
+    "triple_inst_stack
+      (\<langle> h \<le> 1023 \<and> Gverylow \<le> g \<and> m \<ge> 0\<rangle> \<and>*
+       continuing \<and>* memory_usage m \<and>* program_counter n \<and>* data_lst 0 lst \<and>*
+       stack_height (Suc h) \<and>* stack h u \<and>* gas_pred g \<and>* rest)
+      (n, Stack CALLDATALOAD)
+      (program_counter (n + 1) \<and>* continuing \<and>* data_lst 0 lst \<and>*
+       memory_usage m \<and>* stack_height (Suc h) \<and>*
+       stack h (read_word_from_bytes (unat u) lst) \<and>*
+       gas_pred (g - Gverylow) \<and>* rest)"
 
 inductive triple_inst_misc :: "pred \<Rightarrow> pos_inst \<Rightarrow> pred \<Rightarrow> bool" where
  inst_stop :
@@ -195,12 +205,111 @@ inductive triple_inst_misc :: "pred \<Rightarrow> pos_inst \<Rightarrow> pred \<
       (stack_height h \<and>* not_continuing \<and>* memory_usage m \<and>*
        program_counter n \<and>* action (ContractReturn []) \<and>*
        gas_pred g \<and>* rest)"
+|inst_return :
+    "triple_inst_misc
+      (\<langle> h \<le> 1024 \<and> 0 \<le> g \<and> m \<ge> 0 \<and> length lst = unat v\<rangle> \<and>* continuing \<and>* memory_usage m \<and>*
+       program_counter n \<and>* stack_height h \<and>* gas_pred g \<and>* 
+       (if h \<ge> 2 then stack (h-1) u \<and>* stack (h-2) v \<and>* memory_range u lst else emp) \<and>*
+       rest)
+      (n, Misc RETURN)
+      (stack_height h \<and>* not_continuing \<and>* memory_usage m \<and>*
+       action (ContractReturn (if h \<ge> 2 then lst else [])) \<and>*
+       (if h \<ge> 2 then stack (h-1) u \<and>* stack (h-2) v \<and>* memory_range u lst else emp) \<and>*
+       program_counter n \<and>* gas_pred g \<and>* rest)"
+
+definition memory :: "w256 \<Rightarrow> w256 \<Rightarrow> state_element set_pred" where
+"memory ind w = memory_range ind (word_rsplit w)"
+
+definition gcopy_aux :: "w256 \<Rightarrow> int" where
+"gcopy_aux s = (Gcopy * (Word.uint s +( 31 :: int)) div( 32 :: int))"
+
+definition w8_of_inst :: "inst \<Rightarrow> byte" where
+"w8_of_inst inst =
+    (case  index (inst_code inst)(( 0 :: nat)) of
+      None =>(((word_of_int 0) ::  8 word))
+    | Some a => a
+    )"
+
+definition code_range_minus_current_inst :: "int \<Rightarrow> inst list \<Rightarrow> int \<Rightarrow> state_element set \<Rightarrow> bool" where
+"code_range_minus_current_inst src insts n = 
+  (if src \<le> n \<and> n \<le> src + (sum_list (map inst_size insts))
+    then code_range src (take (nat (n - src)) insts) \<and>* code_range (n+1) (drop (nat (n+1)) insts)
+    else code_range src insts)"
+
+inductive triple_inst_memory :: "pred \<Rightarrow> pos_inst \<Rightarrow> pred \<Rightarrow> bool" where
+ inst_mload :
+    "triple_inst_memory
+      (\<langle> h \<le> 1023  \<and> g \<ge> Gverylow + Cmem memu - Cmem (M memu memaddr 32) \<and> memu \<ge> 0 \<rangle> \<and>*
+       stack h memaddr \<and>* stack_height (h+1) \<and>* program_counter n \<and>*   
+       memory_usage memu \<and>* memory memaddr v \<and>* gas_pred g \<and>* continuing \<and>* rest)
+     (n, Memory MLOAD)
+    (program_counter (n + 1) \<and>* stack_height (h + 1) \<and>* stack h v \<and>*
+     memory memaddr v \<and>* memory_usage (M memu memaddr 32) \<and>*
+     gas_pred (g - Gverylow + Cmem memu - Cmem (M memu memaddr 32)) \<and>*
+     continuing \<and>* rest)"
+| inst_mstore :
+    "triple_inst_memory
+      (\<langle> h \<le> 1022 \<and> g \<ge> Gverylow - Cmem memu + Cmem (M memu memaddr 32) \<and> memu \<ge> 0\<rangle> \<and>*
+       stack (h+1) memaddr \<and>* stack h v \<and>* stack_height (h+2) \<and>*
+       program_counter n \<and>* memory_usage memu \<and>*
+       memory memaddr old_v \<and>* gas_pred g \<and>* continuing \<and>* rest)
+      (n, Memory MSTORE)
+      (program_counter (n + 1) \<and>* stack_height h \<and>* memory memaddr v \<and>* 
+       gas_pred (g - Gverylow + Cmem memu - Cmem (M memu memaddr 32)) \<and>*
+       memory_usage (M memu memaddr 32) \<and>* continuing \<and>* rest)"
+| inst_codecopy :
+      "triple_inst_memory
+        (\<langle>h \<le> 1021 \<and> g \<ge> Gverylow + gcopy_aux len \<and> m \<ge> 0 \<and> length lst = unat len \<and>
+         length xs = (if nat m > unat dst_start + unat len then unat len else nat m - unat dst_start)\<rangle> \<and>*
+         program_counter n \<and>* continuing \<and>* gas_pred g \<and>* stack_height (Suc (Suc (Suc h))) \<and>*
+         stack h len \<and>* stack (Suc h) src_start \<and>* stack (Suc (Suc h)) dst_start \<and>*
+         memory_range dst_start xs \<and>*
+         code_range (uint dst_start) lst \<and>* memory_usage m \<and>* rest)
+        (n, Memory CODECOPY)
+        (program_counter (n+1) \<and>* continuing \<and>* gas_pred (g - Gverylow - gcopy_aux u) \<and>*
+         stack_height h \<and>* memory_range dst_start (map w8_of_inst lst) \<and>*
+         code_range (uint dst_start) lst \<and>* memory_usage m \<and>* rest)"
+
+inductive triple_inst_info :: "pred \<Rightarrow> pos_inst \<Rightarrow> pred \<Rightarrow> bool" where
+ inst_callvalue:
+    "triple_inst_info
+      (\<langle> h \<le> 1023 \<and> Gbase \<le> g \<and> m \<ge> 0\<rangle> \<and>*
+       continuing \<and>* program_counter n \<and>*
+       memory_usage m \<and>* stack_height h \<and>* sent_value w \<and>*
+       gas_pred g \<and>* rest)
+      (n, Info CALLVALUE)
+      (program_counter (n + 1) \<and>*
+       continuing \<and>* memory_usage m \<and>* sent_value w \<and>*
+       stack_height (Suc h) \<and>* gas_pred (g - Gbase) \<and>*
+       stack h w \<and>* rest)"
+
+definition new_log_entry :: "address \<Rightarrow> w256 list \<Rightarrow> byte list \<Rightarrow> log_entry"
+where
+"new_log_entry addr topics data = \<lparr>log_addr = addr, log_topics = topics, log_data = data \<rparr>"
+
+inductive triple_inst_log :: "pred \<Rightarrow> pos_inst \<Rightarrow> pred \<Rightarrow> bool" where
+ inst_log0:
+    "triple_inst_log
+    (\<langle>h\<le> 1022 \<and> g \<ge> (Glog + Glogdata * (uint u)) \<and> m \<ge> 0 \<and> length lst = unat u\<rangle> \<and>*
+     program_counter n \<and>* gas_pred g \<and>* memory_usage m \<and>* memory_range v lst \<and>*
+     stack h u \<and>* stack (Suc h) v \<and>* stack_height (Suc (Suc h)) \<and>*
+     log_number l \<and>* continuing \<and>* this_account addr \<and>* rest)
+    (n, Log LOG0)
+    (program_counter (n+1) \<and>* gas_pred (g - (Glog + Glogdata * (uint u))) \<and>* memory_usage m \<and>*
+     stack_height h \<and>* log_number (Suc l) \<and>* logged l (new_log_entry addr [] lst) \<and>*
+     memory_range v lst \<and>* continuing \<and>* this_account addr \<and>* rest)"
 
 inductive triple_inst :: "pred \<Rightarrow> pos_inst \<Rightarrow> pred \<Rightarrow> bool" where
   inst_arith :
     "triple_inst_arith p (n, Arith i) q \<Longrightarrow> triple_inst p (n, Arith i) q"
 | inst_bits :
     "triple_inst_bits p (n, Bits i) q \<Longrightarrow> triple_inst p (n, Bits i) q"
+| inst_info :
+    "triple_inst_info p (n, Info i) q \<Longrightarrow> triple_inst p (n, Info i) q"
+| inst_log :
+    "triple_inst_log p (n, Log i) q \<Longrightarrow> triple_inst p (n, Log i) q"
+| inst_memory :
+    "triple_inst_memory p (n, Memory i) q \<Longrightarrow> triple_inst p (n, Memory i) q"
 | inst_misc :
     "triple_inst_misc p (n, Misc i) q \<Longrightarrow> triple_inst p (n, Misc i) q"
 | inst_pc :
@@ -209,14 +318,24 @@ inductive triple_inst :: "pred \<Rightarrow> pos_inst \<Rightarrow> pred \<Right
     "triple_inst_stack p (n, Stack i) q \<Longrightarrow> triple_inst p (n, Stack i) q"
 | inst_swap :
 		"triple_inst
-			(\<langle> h \<le> 1024 \<and> Suc (unat n) < h \<and> g \<ge> Gverylow \<and> m \<ge> 0\<rangle> **
-			 stack_height h ** stack (h - 1) w ** stack (h - (unat n) - 2) v **
-			 program_counter k ** gas_pred g ** memory_usage m **
-			 continuing ** rest)
+			(\<langle> h \<le> 1024 \<and> Suc (unat n) < h \<and> g \<ge> Gverylow \<and> m \<ge> 0\<rangle> \<and>*
+			 stack_height h \<and>* stack (h - 1) w \<and>* stack (h - (unat n) - 2) v \<and>*
+			 program_counter k \<and>* gas_pred g \<and>* memory_usage m \<and>*
+			 continuing \<and>* rest)
 			(k, Swap n)
-			(program_counter (k + 1) ** gas_pred (g - Gverylow) **
-			 stack_height h ** stack (h - 1) v ** stack (h - (unat n) - 2) w **
-			 memory_usage m ** continuing ** rest)"
+			(program_counter (k + 1) \<and>* gas_pred (g - Gverylow) \<and>*
+			 stack_height h \<and>* stack (h - 1) v \<and>* stack (h - (unat n) - 2) w \<and>*
+			 memory_usage m \<and>* continuing \<and>* rest)"
+| inst_dup :
+    "triple_inst
+      (\<langle> h \<le> 1023 \<and> unat n < h \<and> g \<ge> Gverylow\<rangle> \<and>*
+       stack_height h \<and>* stack (h - (unat n) - 1) w \<and>*
+       memory_usage m \<and>* program_counter k \<and>*
+       gas_pred g \<and>* continuing \<and>* rest )
+      (k, Dup n)
+      (program_counter (k + 1) \<and>* gas_pred (g - Gverylow) \<and>*
+       stack_height (h + 1) \<and>* stack (h - (unat n) - 1) w \<and>* stack h w \<and>*
+       memory_usage m \<and>* continuing \<and>* rest )"
 | inst_strengthen_pre:
     "triple_inst p i q \<Longrightarrow> (\<And>s. r s \<Longrightarrow> p s) \<Longrightarrow> triple_inst r i q"
 | inst_false_pre:
